src/OCL_tools.thy
@@ -69,7 +69,7 @@ lemmas substs4 = OCL_core.StrongEq_L_subst4_rev
                  
 lemmas substs = substs1 substs2 substs4 [THEN iffD2] substs4
 thm substs
-thm  OCL_core.foundation20
+thm  OCL_core.foundation20 
 find_theorems "_ \<Turnstile> \<delta> _"
 ML{*
 fun ocl_subst_asm_tac ctxt  = FIRST'(map (fn C => (etac C) THEN' (simp_tac ctxt)) 
@@ -107,25 +107,14 @@ by(ocl_subst_asm, simp)
 lemma test7 : "\<not> (\<tau> \<Turnstile> (\<upsilon> A)) \<Longrightarrow> \<tau> \<Turnstile> (not B) \<Longrightarrow> \<not> (\<tau> \<Turnstile> (A and B))"
 by(ocl_subst_asm,ocl_subst_asm,simp)
 
-
-lemma bool_split': "(\<tau> \<Turnstile> \<upsilon> A) = ((\<tau> \<Turnstile> A \<triangleq> null) \<or> (\<tau> \<Turnstile> A) \<or> (\<tau> \<Turnstile> not A)) "
-apply(insert bool_split[of A \<tau>], simp add: foundation18, elim disjE, simp_all)
-apply(simp add:OclValid_def StrongEq_def)
-apply(simp_all add:true_def false_def invalid_def null_def null_fun_def null_option_def bot_option_def OclValid_def OclNot_def)
-apply(simp_all add:StrongEq_def)
-done
-
-
-lemma bool_split'': "(\<tau> \<Turnstile> \<delta> A) = ((\<tau> \<Turnstile> A) \<or> (\<tau> \<Turnstile> not A))"
-apply(auto simp:OCL_core.foundation16')
-apply(insert foundation8[of \<tau> A], auto)
-apply(auto simp:true_def false_def invalid_def null_def null_fun_def null_option_def bot_option_def OclValid_def OclNot_def)
-done
+                  
+    
 
 
 (* a proof that shows that not everything is humpty dumpty ... *)
 lemma X: "\<not> (\<tau> \<Turnstile> (invalid and B))"
-apply(insert OCL_core.foundation8[of "\<tau>" "B"], elim disjE, simp add:bool_split'', elim disjE)
+apply(insert OCL_core.foundation8[of "\<tau>" "B"], elim disjE, 
+      simp add:defined_bool_split, elim disjE)
 apply(ocl_subst_asm, simp)
 apply(ocl_subst_asm, simp)
 apply(ocl_subst_asm, simp)
